Denot.v
@@ -1,0 +1,130 @@
+From ITree Require Import
+     ITree.
+
+From ExtLib Require Import
+     Maps
+     FMapAList
+     RelDec
+     Nat
+     String
+     Monad
+     Traversable.
+
+From Coq Require Import
+     String
+     Nat
+     Arith
+     Relations.
+
+Import ITreeNotations.
+Import MonadNotation.
+Local Open Scope monad_scope.
+Local Open Scope string_scope.
+
+Module Denot.
+  Parameter uid: Set. (** Principal *)
+  Parameter BS: Set. (** ByteString *)
+  Definition var : Set := string.
+  Definition channel (T: Type) := nat.
+
+  (** These types should be used instead of Type, to
+      allow induction on type derivation proofs *)
+  Inductive type :Set :=
+  | TBool: type
+  | TNum: type
+  | TUid: type
+  | TChannel: type -> type
+  | TBytestring: type
+  | TUnit: type
+  | TArr: type -> type -> type.
+  
+  Fixpoint typeDenote(t: type): Set :=
+    match t with
+    | TBool => bool
+    | TNum => nat
+    | TUid => uid
+    | TChannel a => channel (typeDenote a)
+    | TBytestring => BS
+    | TUnit => unit
+    | TArr a b => typeDenote a -> typeDenote b
+    end.
+
+  Coercion typeDenote: type >-> Sortclass.
+
+  (** Ghost types *)
+  Definition Enc (p: uid) := BS.
+  Definition Sig (p: uid) := BS.
+  Definition Pub (p: uid) := BS.
+  Definition Priv (p: uid) := BS.
+
+  Declare Custom Entry ty.
+  Notation "<{{ e }}>" := e (e custom ty at level 99).
+  Notation "( x )" := x (in custom ty, x at level 99).
+  Notation "x" := x (in custom ty at level 0, x constr at level 0).
+  Notation "S -> T" := (TArr S T) (in custom ty at level 2, right associativity).
+  Notation "'Num'" := TNum (in custom ty at level 0).
+  Notation "'Bool'" := TBool (in custom ty at level 0).
+  Notation "'Bytestring'" := TBytestring (in custom ty at level 0).
+  Notation "'Channel' T" := (TChannel T) (in custom ty at level 1).
+  Notation "'UID'" := (TUid) (in custom ty at level 0).
+  Notation "'Unit'" := TUnit (in custom ty at level 0).
+
+  Inductive Msg := mkMsg (principal: uid)(payload: BS).
+  
+  (** High-level PKI lang *)
+  Inductive PKI: Type -> Type :=
+  | EncPub(p: uid)(k: Pub p)(plain: BS): PKI (Enc p)
+  | DecPriv(p: uid)(k: Priv p)(cipher: Enc p): PKI BS
+  | SignPriv(p: uid)(k: Priv p)(plain: BS): PKI (Sig p)
+  | CheckPub(p: uid)(k: Pub p)(signed: Sig p): PKI bool.
+
+  (** High-level network lang *)
+  Inductive Net: Type -> Type := (** blocking *)
+  | Recv: Net Msg 
+  | Send : Msg -> Net unit.
+
+  (** High-level Storage lang *)
+  Inductive Storage : Type -> Type :=
+  | Load: var -> Storage nat
+  | Store : var -> nat -> Storage unit.
+  
+  (** High-level parallezation lang (similar to Go channels) *)
+  Inductive spawnE E : Type -> Type :=
+  | Spawn : forall T (c: channel T) (t: itree (spawnE E +' E) T), spawnE E (channel T)
+  | Make: forall (t: type), spawnE E (channel (typeDenote t))
+  | Block: forall T (c: channel T), spawnE E T.
+  
+  Notation Sys := (spawnE (PKI +' Net +' Storage)) (only parsing).
+
+  Definition load := embed Load.
+  Definition store := embed Store.
+  Definition recv := embed Recv.
+  Definition send := embed Send.
+  Definition encrypt := embed EncPub.
+  Definition decrypt := embed DecPriv.
+  Definition sign := embed SignPriv.
+  Definition check := embed CheckPub.
+  
+  
+  Definition make {F E} `{(spawnE F) -< E} (t: type): itree E (channel t) :=
+    trigger (Make F t).
+
+  Definition spawn {F E T} `{(spawnE F) -< E} (c: channel T)(t:itree (spawnE F +' F) T) : itree E (channel T) :=
+    trigger (Spawn F T c t).
+  
+  Definition block := embed Block.
+
+  Set Implicit Arguments.
+
+  Definition example : itree Storage unit :=
+    store "a" 1 ;;
+    n <- load "a" ;;
+    store "a" (n + 1).
+
+  Definition example' : itree Sys unit :=
+    c <- make <{{ Num }}> ;; 
+    store "a" 1 ;;
+    n <- load "a" ;;
+    store "a" (n + 1).
+
+End Denot.
