Utilities.v
@@ -1,0 +1,86 @@
+From Coq Require Import
+     Relations
+     List.
+
+From ExtLib Require Import
+     Core.RelDec
+     Data.Nat
+     Structures.Maps
+     Structures.Monoid
+     Data.Map.FMapAList.
+
+Import ListNotations.
+
+Set Implicit Arguments.
+
+Module Utilities.
+  Parameter uid : Set.
+  Parameter var : Set.
+  Parameter BS: Set.
+
+  Parameter eqdec_var: RelDec (@eq var).
+  Parameter eqdec_uid: RelDec (@eq uid).
+  Parameter eqdec_BS: RelDec (@eq BS).
+
+  Global Existing Instance eqdec_var.
+  Global Existing Instance eqdec_uid.
+  Global Existing Instance eqdec_BS.
+  
+  Inductive primtype: Set :=
+  | TBool: primtype
+  | TNum: primtype
+  | TBytestring: primtype
+  | TUnit: primtype.
+
+  Definition primtypeDenote(t: primtype): Set :=
+    match t with
+    | TBool => bool
+    | TNum => nat
+    | TBytestring => BS
+    | TUnit => unit
+    end.
+
+  Coercion primtypeDenote: primtype >-> Sortclass.
+  Declare Custom Entry ty.
+  Notation "<{{ e }}>" := e (e custom ty at level 99).
+  Notation "( x )" := x (in custom ty, x at level 99).
+  Notation "x" := x (in custom ty at level 0, x constr at level 0).
+  Notation "'Num'" := TNum (in custom ty at level 0).
+  Notation "'Bool'" := TBool (in custom ty at level 0).
+  Notation "'Bytestring'" := TBytestring (in custom ty at level 0).
+  Notation "'Unit'" := TUnit (in custom ty at level 0).
+
+  Parameter serialize: forall (t: primtype), primtypeDenote t -> BS.
+  Parameter deserialize: forall (t: primtype), BS -> primtypeDenote t.
+  
+  Record message := {
+      from: uid;
+      to: uid;
+      t: primtype;
+      payload: primtypeDenote t
+    }.
+
+  Inductive label :=
+  | Msg (m : message)
+  | Silent.
+
+  (** State := my own uid and a valuation context (heap) *)
+  Notation local := (uid * alist var BS)%type (only parsing).
+  
+  (** Backwards *)
+  Inductive trsys A (R: A -> A -> Prop): relation A :=
+  | refl: forall a, trsys R a a
+  | trans: forall a b c, 
+      trsys R a b ->
+      R b c ->
+      trsys R a c.
+
+  Inductive trsys_label A (R: A -> label -> A -> Prop): list label -> relation A :=
+  | reflL: forall a, trsys_label R [] a a
+  | transL: forall a b c h tr, R a h b ->
+                         trsys_label R tr b c ->
+                         trsys_label R (h :: tr) a c.
+
+  Global Hint Constructors label trsys_label trsys: core.
+
+End Utilities.
